Restructure proofs and annotate with descriptions

isabelle/Insert_Spec.thy
@@ -1,6 +1,25 @@
+(* Martin Kleppmann, University of Cambridge
+   Victor B. F. Gomes, University of Cambridge
+   Dominic P. Mulligan, Arm Research, Cambridge
+*)
+
+section\<open>Specifying list insertion\<close>
+
 theory Insert_Spec
   imports OpSet
 begin
+
+text\<open>In this section we consider only list insertion. We model an insertion
+operation as a pair (ID, ref), where ref is either ``None'' (signifying an
+insertion at the head of the list) or ``Some r'' (an insertion immediately
+after a reference element with ID ``r''). If the reference element does not
+exist, the operation does nothing.
+
+We provide two different definitions of the interpretation function for list
+insertion: insert\_spec and insert\_alt. The insert\_alt definition matches
+the paper, while insert\_spec uses the Isabelle/HOL list datatype, making it
+more suitable for formal reasoning. In a later subsection we prove that the
+two definitions are in fact equivalent.\<close>
 
 fun insert_spec :: "'oid list \<Rightarrow> ('oid \<times> 'oid option) \<Rightarrow> 'oid list" where
   "insert_spec xs     (oid, None)     = oid#xs" |
@@ -9,13 +28,35 @@ fun insert_spec :: "'oid list \<Rightarrow> ('oid \<times> 'oid option) \<Righta
      (if x = ref then x # oid # xs
                  else x # (insert_spec xs (oid, Some ref)))"
 
+fun insert_alt :: "('oid \<times> 'oid option) set \<Rightarrow> ('oid \<times> 'oid) \<Rightarrow> ('oid \<times> 'oid option) set" where
+  "insert_alt list_rel (oid, ref) = (
+      if \<exists>n. (ref, n) \<in> list_rel
+      then {(p, n) \<in> list_rel. p \<noteq> ref} \<union> {(ref, Some oid)} \<union>
+           {(i, n). i = oid \<and> (ref, n) \<in> list_rel}
+      else list_rel)"
+
+text\<open>The make\_insert function generates a new operation for insertion into
+a given index in a given list.\<close>
+
 fun make_insert :: "'oid list \<Rightarrow> 'oid \<Rightarrow> nat \<Rightarrow> ('oid \<times> 'oid option)" where
   "make_insert xs oid 0       = (oid, None)" |
   "make_insert [] oid m       = (oid, None)" |
   "make_insert xs oid (Suc m) = (oid, Some (xs ! min (length xs - 1) m))"
 
+text\<open>interp\_list is the sequential interpretation of a set of insertion
+operations. It starts with an empty list as initial state, and then applies
+the operations from left to right.\<close>
+
 definition interp_list :: "('oid \<times> 'oid option) list \<Rightarrow> 'oid list" where
   "interp_list ops \<equiv> foldl insert_spec [] ops"
+
+
+subsection \<open>The insert\_ops predicate\<close>
+
+text\<open>We now specialise the definitions from the abstract OpSet section for list
+insertion. insert\_opset is an opset consisting only of insertion operations,
+and insert\_ops is the specialisation of the spec\_ops predicate for
+insertion operations. We prove several useful lemmas about insert\_ops.\<close>
 
 locale insert_opset = opset opset set_option
   for opset :: "('oid::{linorder} \<times> 'oid option) set"
@@ -78,7 +119,7 @@ lemma insert_ops_memb_ref_older:
 using assms insert_ops_ref_older split_list_first by fastforce
 
 
-subsection \<open>Properties of the insert_spec function\<close>
+subsection \<open>Properties of the insert\_spec function\<close>
 
 lemma insert_spec_none [simp]:
   shows "set (insert_spec xs (oid, None)) = set xs \<union> {oid}"
@@ -141,11 +182,11 @@ qed
 
 lemma insert_spec_distinct [intro]:
   fixes oid :: "'oid::{linorder}"
-  assumes 1: "distinct xs"
-    and 2: "\<And>x. x \<in> set xs \<Longrightarrow> x < oid"
-    and 3: "ref = Some r \<longrightarrow> r < oid"
+  assumes "distinct xs"
+    and "\<And>x. x \<in> set xs \<Longrightarrow> x < oid"
+    and "ref = Some r \<longrightarrow> r < oid"
   shows "distinct (insert_spec xs (oid, ref))"
-using 1 2 proof(induction xs)
+using assms(1) assms(2) proof(induction xs)
   show "distinct (insert_spec [] (oid, ref))"
     by(cases ref, auto)
 next
@@ -193,30 +234,31 @@ next
 qed
 
 lemma insert_after_ref:
-  assumes "distinct (xs@ref#ys)"
-  shows "insert_spec (xs@ref#ys) (oid, Some ref) = xs@ref#oid#ys"
+  assumes "distinct (xs @ ref # ys)"
+  shows "insert_spec (xs @ ref # ys) (oid, Some ref) = xs @ ref # oid # ys"
 using assms by (induction xs, auto)
 
 lemma insert_somewhere:
   assumes "ref = None \<or> (ref = Some r \<and> r \<in> set list)"
-  shows "\<exists>xs ys. list = xs@ys \<and> insert_spec list (oid, ref) = xs@oid#ys"
+  shows "\<exists>xs ys. list = xs @ ys \<and> insert_spec list (oid, ref) = xs @ oid # ys"
 using assms proof(induction list)
   assume "ref = None \<or> ref = Some r \<and> r \<in> set []"
   thus "\<exists>xs ys. [] = xs @ ys \<and> insert_spec [] (oid, ref) = xs @ oid # ys"
   proof
     assume "ref = None"
-    thus "\<exists>xs ys. [] = xs@ys \<and> insert_spec [] (oid, ref) = xs@oid#ys"
+    thus "\<exists>xs ys. [] = xs @ ys \<and> insert_spec [] (oid, ref) = xs @ oid # ys"
       by auto
   next
     assume "ref = Some r \<and> r \<in> set []"
-    thus "\<exists>xs ys. [] = xs@ys \<and> insert_spec [] (oid, ref) = xs@oid#ys"
+    thus "\<exists>xs ys. [] = xs @ ys \<and> insert_spec [] (oid, ref) = xs @ oid # ys"
       by auto
   qed
 next
   fix a list
   assume 1: "ref = None \<or> ref = Some r \<and> r \<in> set (a#list)"
-    and IH: "ref = None \<or> ref = Some r \<and> r \<in> set list \<Longrightarrow> \<exists>xs ys. list = xs@ys \<and> insert_spec list (oid, ref) = xs@oid#ys"
-  show "\<exists>xs ys. a#list = xs@ys \<and> insert_spec (a#list) (oid, ref) = xs@oid#ys"
+    and IH: "ref = None \<or> ref = Some r \<and> r \<in> set list \<Longrightarrow>
+         \<exists>xs ys. list = xs @ ys \<and> insert_spec list (oid, ref) = xs @ oid # ys"
+  show "\<exists>xs ys. a # list = xs @ ys \<and> insert_spec (a # list) (oid, ref) = xs @ oid # ys"
   proof(rule disjE[OF 1])
     assume "ref = None"
     thus "\<exists>xs ys. a # list = xs @ ys \<and> insert_spec (a # list) (oid, ref) = xs @ oid # ys"
@@ -232,7 +274,8 @@ next
         using 3 by(metis append_Cons append_Nil insert_spec.simps(3))
     next
       assume "r \<in> set list"
-      from this obtain xs ys where "list = xs@ys \<and> insert_spec list (oid, ref) = xs@oid#ys"
+      from this obtain xs ys
+        where "list = xs @ ys \<and> insert_spec list (oid, ref) = xs @ oid # ys"
         using IH 3 by auto
       thus "\<exists>xs ys. a # list = xs @ ys \<and> insert_spec (a # list) (oid, ref) = xs @ oid # ys"
         using 3 by clarsimp (metis append_Cons append_Nil)
@@ -293,7 +336,7 @@ next
 qed
 
 
-subsection \<open>Properties of the interp_list function\<close>
+subsection \<open>Properties of the interp\_list function\<close>
 
 lemma interp_list_empty [simp]:
   shows "interp_list [] = []"
@@ -350,38 +393,307 @@ next
     by (simp add: x_pair interp_list_tail_unfold)
 qed
 
-lemma distinct_list_split:
-  assumes "distinct xs"
-    and "xs = xa @ x # ya"
-    and "xs = xb @ x # yb"
-  shows "xa = xb \<and> ya = yb"
-using assms proof(induction xs arbitrary: xa xb x)
-  fix xa xb x
-  assume "[] = xa @ x # ya"
-  thus "xa = xb \<and> ya = yb"
-    by auto
+
+subsection \<open>Equivalence of the two definitions of insertion\<close>
+
+text\<open>At the beginning of this section we gave two different definitions of
+interpretation functions for list insertion: insert\_spec and insert\_alt.
+In this section we prove that the two are equivalent.
+
+We first define how to derive the successor relation from an Isabelle list.
+This relation contains (\emph{id}, None) if \emph{id} is the last element
+of the list, and (\emph{id1}, \emph{id2}) if \emph{id1} is immediately
+followed by \emph{id2} in the list.\<close>
+
+fun succ_rel :: "'oid list \<Rightarrow> ('oid \<times> 'oid option) set" where
+  "succ_rel [] = {}" |
+  "succ_rel [head] = {(head, None)}" |
+  "succ_rel (head#x#xs) = {(head, Some x)} \<union> succ_rel (x#xs)"
+
+text\<open>interp\_alt is the equivalent of interp\_list, but using insert\_alt
+instead of insert\_spec. To match the paper, it uses a distinct head element
+to refer to the beginning of the list.\<close>
+
+definition interp_alt :: "'oid \<Rightarrow> ('oid \<times> 'oid option) list \<Rightarrow> ('oid \<times> 'oid option) set" where
+  "interp_alt head ops \<equiv> foldl insert_alt {(head, None)}
+     (map (\<lambda>x. case x of
+            (oid, None)     \<Rightarrow> (oid, head) |
+            (oid, Some ref) \<Rightarrow> (oid, ref)) 
+      ops)"
+
+lemma succ_rel_set_fst:
+  shows "fst ` (succ_rel xs) = set xs"
+by (induction xs rule: succ_rel.induct, auto)
+
+lemma succ_rel_functional:
+  assumes "(a, b1) \<in> succ_rel xs"
+    and "(a, b2) \<in> succ_rel xs"
+    and "distinct xs"
+  shows "b1 = b2"
+using assms proof(induction xs rule: succ_rel.induct)
+  case 1
+  then show ?case by simp
 next
-  fix a xs xa xb x
-  assume IH: "\<And>xa xb x. distinct xs \<Longrightarrow> xs = xa @ x # ya \<Longrightarrow> xs = xb @ x # yb \<Longrightarrow> xa = xb \<and> ya = yb"
-    and "distinct (a # xs)" and "a # xs = xa @ x # ya" and "a # xs = xb @ x # yb"
-  thus "xa = xb \<and> ya = yb"
-    by(case_tac xa; case_tac xb) auto
+  case (2 head)
+  then show ?case by simp
+next
+  case (3 head x xs)
+  then show ?case
+  proof(cases "a = head")
+    case True
+    hence "a \<notin> set (x#xs)"
+      using 3 by auto
+    hence "a \<notin> fst ` (succ_rel (x#xs))"
+      using succ_rel_set_fst by metis
+    then show "b1 = b2"
+      using 3 image_iff by fastforce
+  next
+    case False
+    hence "{(a, b1), (a, b2)} \<subseteq> succ_rel (x#xs)"
+      using 3 by auto
+    moreover have "distinct (x#xs)"
+      using 3 by auto
+    ultimately show "b1 = b2"
+      using "3.IH" by auto
+  qed
+qed
+
+lemma succ_rel_rem_head:
+  assumes "distinct (x # xs)"
+  shows "{(p, n) \<in> succ_rel (x # xs). p \<noteq> x} = succ_rel xs"
+proof -
+  have head_notin: "x \<notin> fst ` succ_rel xs"
+    using assms by (simp add: succ_rel_set_fst)
+  moreover obtain y where "(x, y) \<in> succ_rel (x # xs)"
+    by (cases xs, auto)
+  moreover have "succ_rel (x # xs) = {(x, y)} \<union> succ_rel xs"
+    using calculation head_notin image_iff by (cases xs, fastforce+)
+  moreover from this have "\<And>n. (x, n) \<in> succ_rel (x # xs) \<Longrightarrow> n = y"
+    by (metis Pair_inject fst_conv head_notin image_eqI insertE insert_is_Un)
+  hence "{(p, n) \<in> succ_rel (x # xs). p \<noteq> x} = succ_rel (x # xs) - {(x, y)}"
+    by blast
+  moreover have "succ_rel (x # xs) - {(x, y)} = succ_rel xs"
+    using image_iff calculation by fastforce
+  ultimately show "{(p, n) \<in> succ_rel (x # xs). p \<noteq> x} = succ_rel xs"
+    by simp
+qed
+
+lemma succ_rel_swap_head:
+  assumes "distinct (ref # list)"
+    and "(ref, n) \<in> succ_rel (ref # list)"
+  shows "succ_rel (oid # list) = {(oid, n)} \<union> succ_rel list"
+proof(cases list)
+  case Nil
+  then show ?thesis using assms by auto
+next
+  case (Cons a list)
+  moreover from this have "n = Some a"
+    by (metis Un_iff assms singletonI succ_rel.simps(3) succ_rel_functional)
+  ultimately show ?thesis by simp
+qed
+
+lemma succ_rel_insert_alt:
+  assumes "a \<noteq> ref"
+    and "distinct (oid # a # b # list)"
+  shows "insert_alt (succ_rel (a # b # list)) (oid, ref) =
+         {(a, Some b)} \<union> insert_alt (succ_rel (b # list)) (oid, ref)"
+proof(cases "\<exists>n. (ref, n) \<in> succ_rel (a # b # list)")
+  case True
+  hence "insert_alt (succ_rel (a # b # list)) (oid, ref) =
+           {(p, n) \<in> succ_rel (a # b # list). p \<noteq> ref} \<union> {(ref, Some oid)} \<union>
+           {(i, n). i = oid \<and> (ref, n) \<in> succ_rel (a # b # list)}"
+    by simp
+  moreover have "{(p, n) \<in> succ_rel (a # b # list). p \<noteq> ref} =
+                 {(a, Some b)} \<union> {(p, n) \<in> succ_rel (b # list). p \<noteq> ref}"
+    using assms(1) by auto
+  moreover have "insert_alt (succ_rel (b # list)) (oid, ref) =
+           {(p, n) \<in> succ_rel (b # list). p \<noteq> ref} \<union> {(ref, Some oid)} \<union>
+           {(i, n). i = oid \<and> (ref, n) \<in> succ_rel (b # list)}"
+  proof -
+    have "\<exists>n. (ref, n) \<in> succ_rel (b # list)"
+      using assms(1) True by auto
+    thus ?thesis by simp
+  qed
+  moreover have "{(i, n). i = oid \<and> (ref, n) \<in> succ_rel (a # b # list)} =
+                 {(i, n). i = oid \<and> (ref, n) \<in> succ_rel (b # list)}"
+    using assms(1) by auto
+  ultimately show ?thesis by simp
+next
+  case False
+  then show ?thesis by auto
+qed
+
+lemma succ_rel_insert_head:
+  assumes "distinct (ref # list)"
+  shows "succ_rel (insert_spec (ref # list) (oid, Some ref)) =
+         insert_alt (succ_rel (ref # list)) (oid, ref)"
+proof -
+  obtain n where ref_in_rel: "(ref, n) \<in> succ_rel (ref # list)"
+    by (cases list, auto)
+  moreover from this have "{(p, n) \<in> succ_rel (ref # list). p \<noteq> ref} = succ_rel list"
+    using assms succ_rel_rem_head by (metis (mono_tags, lifting))
+  moreover have "{(i, n). i = oid \<and> (ref, n) \<in> succ_rel (ref # list)} = {(oid, n)}"
+  proof -
+    have "\<And>nx. (ref, nx) \<in> succ_rel (ref # list) \<Longrightarrow> nx = n"
+      using assms by (simp add: succ_rel_functional ref_in_rel)
+    hence "{(i, n) \<in> succ_rel (ref # list). i = ref} \<subseteq> {(ref, n)}"
+      by blast
+    moreover have "{(ref, n)} \<subseteq> {(i, n) \<in> succ_rel (ref # list). i = ref}"
+      by (simp add: ref_in_rel)
+    ultimately show ?thesis by blast
+  qed
+  moreover have "insert_alt (succ_rel (ref # list)) (oid, ref) =
+                   {(p, n) \<in> succ_rel (ref # list). p \<noteq> ref} \<union> {(ref, Some oid)} \<union>
+                   {(i, n). i = oid \<and> (ref, n) \<in> succ_rel (ref # list)}"
+  proof -
+    have "\<exists>n. (ref, n) \<in> succ_rel (ref # list)"
+      using ref_in_rel by blast
+    thus ?thesis by simp
+  qed
+  ultimately have "insert_alt (succ_rel (ref # list)) (oid, ref) =
+                   succ_rel list \<union> {(ref, Some oid)} \<union> {(oid, n)}"
+    by simp
+  moreover have "succ_rel (oid # list) = {(oid, n)} \<union> succ_rel list"
+    using assms ref_in_rel succ_rel_swap_head by metis
+  hence "succ_rel (ref # oid # list) = {(ref, Some oid), (oid, n)} \<union> succ_rel list"
+    by auto
+  ultimately show "succ_rel (insert_spec (ref # list) (oid, Some ref)) =
+                   insert_alt (succ_rel (ref # list)) (oid, ref)"
+    by auto
+qed
+
+lemma succ_rel_insert_later:
+  assumes "succ_rel (insert_spec (b # list) (oid, Some ref)) =
+           insert_alt (succ_rel (b # list)) (oid, ref)"
+    and "a \<noteq> ref"
+    and "distinct (a # b # list)"
+  shows "succ_rel (insert_spec (a # b # list) (oid, Some ref)) =
+         insert_alt (succ_rel (a # b # list)) (oid, ref)"
+proof -
+  have "succ_rel (a # b # list) = {(a, Some b)} \<union> succ_rel (b # list)"
+    by simp
+  moreover have "insert_spec (a # b # list) (oid, Some ref) =
+                 a # (insert_spec (b # list) (oid, Some ref))"
+    using assms(2) by simp
+  hence "succ_rel (insert_spec (a # b # list) (oid, Some ref)) =
+         {(a, Some b)} \<union> succ_rel (insert_spec (b # list) (oid, Some ref))"
+    by auto
+  hence "succ_rel (insert_spec (a # b # list) (oid, Some ref)) =
+         {(a, Some b)} \<union> insert_alt (succ_rel (b # list)) (oid, ref)"
+    using assms(1) by auto
+  moreover have "insert_alt (succ_rel (a # b # list)) (oid, ref) =
+                 {(a, Some b)} \<union> insert_alt (succ_rel (b # list)) (oid, ref)"
+    using succ_rel_insert_alt assms(2) by auto
+  ultimately show ?thesis by blast
+qed
+
+lemma succ_rel_insert_Some:
+  assumes "distinct list"
+  shows "succ_rel (insert_spec list (oid, Some ref)) = insert_alt (succ_rel list) (oid, ref)"
+using assms proof(induction list)
+  case Nil
+  then show "succ_rel (insert_spec [] (oid, Some ref)) = insert_alt (succ_rel []) (oid, ref)"
+    by simp
+next
+  case (Cons a list)
+  hence "distinct (a # list)"
+    by simp
+  then show "succ_rel (insert_spec (a # list) (oid, Some ref)) =
+             insert_alt (succ_rel (a # list)) (oid, ref)"
+  proof(cases "a = ref")
+    case True
+    then show ?thesis
+      using succ_rel_insert_head \<open>distinct (a # list)\<close> by metis
+  next
+    case False
+    hence "a \<noteq> ref" by simp
+    moreover have "succ_rel (insert_spec list (oid, Some ref)) =
+                   insert_alt (succ_rel list) (oid, ref)"
+      using Cons.IH Cons.prems by auto
+    ultimately show "succ_rel (insert_spec (a # list) (oid, Some ref)) =
+                     insert_alt (succ_rel (a # list)) (oid, ref)"
+      by (cases list, force, metis Cons.prems succ_rel_insert_later)
+  qed
+qed
+
+text\<open>The main result of this section, that insert\_spec and insert\_alt
+are equivalent.\<close>
+
+theorem insert_alt_equivalent:
+  assumes "insert_ops ops"
+    and "head \<notin> fst ` set ops"
+    and "\<And>r. Some r \<in> snd ` set ops \<Longrightarrow> r \<noteq> head"
+  shows "succ_rel (head # interp_list ops) = interp_alt head ops"
+using assms proof(induction ops rule: List.rev_induct)
+  case Nil
+  then show "succ_rel (head # interp_list []) = interp_alt head []"
+    by (simp add: interp_list_def interp_alt_def)
+next
+  case (snoc x xs)
+  have IH: "succ_rel (head # interp_list xs) = interp_alt head xs"
+    using snoc by auto
+  have distinct_list: "distinct (head # interp_list xs)"
+  proof -
+    have "distinct (interp_list xs)"
+      using interp_list_distinct snoc.prems(1) by blast
+    moreover have "set (interp_list xs) \<subseteq> fst ` set xs"
+      using interp_list_subset snoc.prems(1) by fastforce
+    ultimately show "distinct (head # interp_list xs)"
+      using snoc.prems(2) by auto
+  qed
+  obtain oid r where x_pair: "x = (oid, r)" by force
+  then show "succ_rel (head # interp_list (xs @ [x])) = interp_alt head (xs @ [x])"
+  proof(cases r)
+    case None
+    have "interp_alt head (xs @ [x]) = insert_alt (interp_alt head xs) (oid, head)"
+      by (simp add: interp_alt_def None x_pair)
+    moreover have "... = insert_alt (succ_rel (head # interp_list xs)) (oid, head)"
+      by (simp add: IH)
+    moreover have "... = succ_rel (insert_spec (head # interp_list xs) (oid, Some head))"
+      using distinct_list succ_rel_insert_Some by metis
+    moreover have "... = succ_rel (head # (insert_spec (interp_list xs) (oid, None)))"
+      by auto
+    moreover have "... = succ_rel (head # (interp_list (xs @ [x])))"
+      by (simp add: interp_list_tail_unfold None x_pair)
+    ultimately show ?thesis by simp
+  next
+    case (Some ref)
+    have "ref \<noteq> head"
+      by (simp add: Some snoc.prems(3) x_pair)
+    have "interp_alt head (xs @ [x]) = insert_alt (interp_alt head xs) (oid, ref)"
+      by (simp add: interp_alt_def Some x_pair)
+    moreover have "... = insert_alt (succ_rel (head # interp_list xs)) (oid, ref)"
+      by (simp add: IH)
+    moreover have "... = succ_rel (insert_spec (head # interp_list xs) (oid, Some ref))"
+      using distinct_list succ_rel_insert_Some by metis
+    moreover have "... = succ_rel (head # (insert_spec (interp_list xs) (oid, Some ref)))"
+      using \<open>ref \<noteq> head\<close> by auto
+    moreover have "... = succ_rel (head # (interp_list (xs @ [x])))"
+      by (simp add: interp_list_tail_unfold Some x_pair)
+    ultimately show ?thesis by simp
+  qed
 qed
 
 
-subsection \<open>The list_order predicate\<close>
+subsection \<open>The list\_order predicate\<close>
+
+text\<open>``list\_order \emph{ops x y}'' holds iff, after interpreting the list of
+insertion operations \emph{ops}, the list element with ID \emph{x} appears
+before the list element with ID \emph{y} in the resulting list. We prove several
+lemmas about this predicate; in particular, that executing additional insertion
+operations does not change the relative ordering of existing list elements.\<close>
 
 definition list_order :: "('oid::{linorder} \<times> 'oid option) list \<Rightarrow> 'oid \<Rightarrow> 'oid \<Rightarrow> bool" where
-  "list_order ops x y \<equiv> \<exists>xs ys zs. interp_list ops = xs@[x]@ys@[y]@zs"
+  "list_order ops x y \<equiv> \<exists>xs ys zs. interp_list ops = xs @ [x] @ ys @ [y] @ zs"
 
 lemma list_orderI:
-  assumes "interp_list ops = xs@[x]@ys@[y]@zs"
+  assumes "interp_list ops = xs @ [x] @ ys @ [y] @ zs"
   shows "list_order ops x y"
 using assms by (auto simp add: list_order_def)
 
 lemma list_orderE:
   assumes "list_order ops x y"
-  shows "\<exists>xs ys zs. interp_list ops = xs@[x]@ys@[y]@zs"
+  shows "\<exists>xs ys zs. interp_list ops = xs @ [x] @ ys @ [y] @ zs"
 using assms by (auto simp add: list_order_def)
 
 lemma list_order_memb1:
@@ -716,31 +1028,15 @@ using assms proof(induction rule: measure_induct_rule[where f="\<lambda>x. (leng
   qed
 qed
 
-lemma list_split_two_elems:
-  assumes "distinct xs"
-    and "x \<in> set xs" and "y \<in> set xs"
-    and "x \<noteq> y"
-  shows "\<exists>pre mid suf. xs = pre @ x # mid @ y # suf \<or> xs = pre @ y # mid @ x # suf"
-proof -
-  obtain as bs where as_bs: "xs = as @ [x] @ bs"
-    using assms(2) split_list_first by fastforce
-  show ?thesis
-  proof(cases "y \<in> set as")
-    case True
-    then obtain cs ds where "as = cs @ [y] @ ds"
-      using assms(3) split_list_first by fastforce
-    then show ?thesis
-      by (auto simp add: as_bs)
-  next
-    case False
-    then have "y \<in> set bs"
-      using as_bs assms(3) assms(4) by auto
-    then obtain cs ds where "bs = cs @ [y] @ ds"
-      using assms(3) split_list_first by fastforce
-    then show ?thesis
-      by (auto simp add: as_bs)
-  qed
-qed
+
+subsection\<open>Relationship to strong list specification\<close>
+
+text\<open>Attiya et al. \cite{Attiya:2016kh} give a specification of collaborative
+text editing, called $\mathcal{A}_\textsf{strong}$. In this section we prove
+that our specification is stronger than $\mathcal{A}_\textsf{strong}$, by
+showing that whenever an OpSet is interpreted using our list function, the
+outcome satisfies all of the criteria that make up Attiya et al.'s
+specification.\<close>
 
 lemma insert_spec_nth_oid:
   assumes "distinct xs"
@@ -806,6 +1102,32 @@ lemma list_order_transp:
   shows "transp (list_order op_list)"
 using assms list_order_trans transpI by metis
 
+lemma list_split_two_elems:
+  assumes "distinct xs"
+    and "x \<in> set xs" and "y \<in> set xs"
+    and "x \<noteq> y"
+  shows "\<exists>pre mid suf. xs = pre @ x # mid @ y # suf \<or> xs = pre @ y # mid @ x # suf"
+proof -
+  obtain as bs where as_bs: "xs = as @ [x] @ bs"
+    using assms(2) split_list_first by fastforce
+  show ?thesis
+  proof(cases "y \<in> set as")
+    case True
+    then obtain cs ds where "as = cs @ [y] @ ds"
+      using assms(3) split_list_first by fastforce
+    then show ?thesis
+      by (auto simp add: as_bs)
+  next
+    case False
+    then have "y \<in> set bs"
+      using as_bs assms(3) assms(4) by auto
+    then obtain cs ds where "bs = cs @ [y] @ ds"
+      using assms(3) split_list_first by fastforce
+    then show ?thesis
+      by (auto simp add: as_bs)
+  qed
+qed
+
 lemma list_order_total:
   assumes "insert_ops op_list"
     and "x \<in> set (interp_list op_list)"
@@ -827,533 +1149,5 @@ lemma list_order_irrefl:
   assumes 1: "insert_ops op_list"
   shows "\<not> list_order op_list x x"
 using assms interp_list_distinct list_orderE by force
-
-lemma interp_list_maybe_grow:
-  assumes "insert_ops (xs @ [(oid, ref)])"
-  shows "set (interp_list (xs @ [(oid, ref)])) = set (interp_list xs) \<or>
-         set (interp_list (xs @ [(oid, ref)])) = (set (interp_list xs) \<union> {oid})"
-by (cases ref, simp add: interp_list_tail_unfold,
-    metis insert_spec_nonex insert_spec_set interp_list_tail_unfold)
-
-lemma interp_list_maybe_grow2:
-  assumes "insert_ops (xs @ [x])"
-  shows "set (interp_list (xs @ [x])) = set (interp_list xs) \<or>
-         set (interp_list (xs @ [x])) = (set (interp_list xs) \<union> {fst x})"
-using assms interp_list_maybe_grow by (cases x, auto)
-
-lemma interp_list_maybe_grow3:
-  assumes "insert_ops (xs @ ys)"
-  shows "\<exists>A. A \<subseteq> set (map fst ys) \<and> set (interp_list (xs @ ys)) = set (interp_list xs) \<union> A"
-using assms proof(induction ys rule: List.rev_induct)
-  case Nil
-  then show ?case by simp
-next
-  case (snoc x ys)
-  then have "insert_ops (xs @ ys)"
-    by (metis append_assoc insert_ops_rem_last)
-  then obtain A where IH: "A \<subseteq> set (map fst ys) \<and>
-            set (interp_list (xs @ ys)) = set (interp_list xs) \<union> A"
-    using snoc.IH by blast
-  then show ?case
-  proof(cases "set (interp_list (xs @ ys @ [x])) = set (interp_list (xs @ ys))")
-    case True
-    moreover have "A \<subseteq> set (map fst (ys @ [x]))"
-      using IH by auto
-    ultimately show ?thesis
-      using IH by auto
-  next
-    case False
-    then have "set (interp_list (xs @ ys @ [x])) = set (interp_list (xs @ ys)) \<union> {fst x}"
-      by (metis append_assoc interp_list_maybe_grow2 snoc.prems)
-    moreover have "A \<union> {fst x} \<subseteq> set (map fst (ys @ [x]))"
-      using IH by auto
-    ultimately show ?thesis
-      using IH Un_assoc by metis
-  qed
-qed
-
-lemma interp_list_ref_nonex:
-  assumes "insert_ops ops"
-    and "ops = xs @ [(oid, Some ref)] @ ys"
-    and "ref \<notin> set (interp_list xs)"
-  shows "oid \<notin> set (interp_list ops)"
-using assms proof(induction ys arbitrary: ops rule: List.rev_induct)
-  case Nil
-  then have "interp_list ops = insert_spec (interp_list xs) (oid, Some ref)"
-    by (simp add: interp_list_tail_unfold)
-  moreover have "\<And>i. i \<in> set (map fst xs) \<Longrightarrow> i < oid"
-    using Nil.prems last_op_greatest by fastforce
-  hence "\<And>i. i \<in> set (interp_list xs) \<Longrightarrow> i < oid"
-    by (meson interp_list_subset subsetCE)
-  ultimately show "oid \<notin> set (interp_list ops)"
-    using assms(3) by auto
-next
-  case (snoc x ys)
-  then have "insert_ops (xs @ (oid, Some ref) # ys)"
-    by (metis append.assoc append.simps(1) append_Cons insert_ops_appendD)
-  hence IH: "oid \<notin> set (interp_list (xs @ (oid, Some ref) # ys))"
-    by (simp add: snoc.IH snoc.prems(3))
-  moreover have "distinct (map fst (xs @ (oid, Some ref) # ys @ [x]))"
-    using snoc.prems by (metis append_Cons append_self_conv2 insert_ops_def spec_ops_def)
-  hence "fst x \<noteq> oid"
-    using empty_iff by auto
-  moreover have "insert_ops ((xs @ (oid, Some ref) # ys) @ [x])"
-    using snoc.prems by auto
-  hence "set (interp_list ((xs @ (oid, Some ref) # ys) @ [x])) =
-         set (interp_list (xs @ (oid, Some ref) # ys)) \<or> 
-         set (interp_list ((xs @ (oid, Some ref) # ys) @ [x])) =
-         set (interp_list (xs @ (oid, Some ref) # ys)) \<union> {fst x}"
-    using interp_list_maybe_grow2 by blast
-  ultimately show "oid \<notin> set (interp_list ops)"
-    using snoc.prems(2) by auto
-qed
-
-lemma map_fst_append1:
-  assumes "\<forall>i \<in> set (map fst xs). P i"
-    and "P x"
-  shows "\<forall>i \<in> set (map fst (xs @ [(x, y)])). P i"
-using assms by (induction xs, auto)
-
-lemma insert_ops_split:
-  assumes "insert_ops ops"
-    and "(oid, ref) \<in> set ops"
-  shows "\<exists>pre suf. ops = pre @ [(oid, ref)] @ suf \<and>
-            (\<forall>i \<in> set (map fst pre). i < oid) \<and>
-            (\<forall>i \<in> set (map fst suf). oid < i)"
-using assms proof(induction ops rule: List.rev_induct)
-  case Nil
-  then show ?case by auto
-next
-  case (snoc x xs)
-  then show ?case
-  proof(cases "x = (oid, ref)")
-    case True
-    moreover from this have "\<forall>i \<in> set (map fst xs). i < oid"
-      using last_op_greatest snoc.prems(1) by blast
-    ultimately have "xs @ [x] = xs @ [(oid, ref)] @ [] \<and>
-            (\<forall>i \<in> set (map fst xs). i < oid) \<and>
-            (\<forall>i \<in> set (map fst []). oid < i)"
-      by auto
-    then show ?thesis by force
-  next
-    case False
-    hence "(oid, ref) \<in> set xs"
-      using snoc.prems(2) by auto
-    from this obtain pre suf where IH: "xs = pre @ [(oid, ref)] @ suf \<and>
-         (\<forall>i \<in> set (map fst pre). i < oid) \<and>
-         (\<forall>i \<in> set (map fst suf). oid < i)"
-      using snoc.IH snoc.prems(1) by blast
-    obtain xi xr where x_pair: "x = (xi, xr)"
-      by force
-    hence "distinct (map fst (pre @ [(oid, ref)] @ suf @ [(xi, xr)]))"
-      by (metis IH append.assoc insert_ops_def spec_ops_def snoc.prems(1))
-    hence "xi \<noteq> oid"
-      by auto
-    have xi_max: "\<forall>x \<in> set (map fst (pre @ [(oid, ref)] @ suf)). x < xi"
-      using IH last_op_greatest snoc.prems(1) x_pair by blast
-    then show ?thesis
-    proof(cases "xi < oid")
-      case True
-      moreover from this have "\<forall>x \<in> set suf. fst x < oid"
-        using xi_max by auto
-      hence "suf = []"
-        using IH last_in_set by fastforce
-      ultimately have "xs @ [x] = (pre @ [(xi, xr)]) @ [] \<and>
-              (\<forall>i \<in> set (map fst ((pre @ [(xi, xr)]))). i < oid) \<and>
-              (\<forall>i \<in> set (map fst []). oid < i)"
-        using dual_order.asym xi_max by auto
-      then show ?thesis by (simp add: IH)
-    next
-      case False
-      hence "oid < xi"
-        using \<open>xi \<noteq> oid\<close> by auto
-      hence "\<forall>i \<in> set (map fst (suf @ [(xi, xr)])). oid < i"
-        using IH map_fst_append1 by auto
-      hence "xs @ [x] = pre @ [(oid, ref)] @ (suf @ [(xi, xr)]) \<and>
-              (\<forall>i \<in> set (map fst pre). i < oid) \<and>
-              (\<forall>i \<in> set (map fst (suf @ [(xi, xr)])). oid < i)"
-        by (simp add: IH x_pair)
-      then show ?thesis by blast
-    qed
-  qed
-qed
-
-lemma insert_ops_split_2:
-  assumes "insert_ops ops"
-    and "(xid, xr) \<in> set ops"
-    and "(yid, yr) \<in> set ops"
-    and "xid < yid"
-  shows "\<exists>as bs cs. ops = as @ [(xid, xr)] @ bs @ [(yid, yr)] @ cs \<and>
-           (\<forall>i \<in> set (map fst as). i < xid) \<and>
-           (\<forall>i \<in> set (map fst bs). xid < i \<and> i < yid) \<and>
-           (\<forall>i \<in> set (map fst cs). yid < i)"
-proof -
-  obtain as as1 where x_split: "ops = as @ [(xid, xr)] @ as1 \<and>
-      (\<forall>i \<in> set (map fst as). i < xid) \<and> (\<forall>i \<in> set (map fst as1). xid < i)"
-    using assms insert_ops_split by blast
-  hence "insert_ops ((as @ [(xid, xr)]) @ as1)"
-    using assms(1) by auto
-  hence "insert_ops as1"
-    using assms(1) insert_ops_rem_prefix by blast
-  have "(yid, yr) \<in> set as1"
-    using x_split assms by auto
-  from this obtain bs cs where y_split: "as1 = bs @ [(yid, yr)] @ cs \<and>
-      (\<forall>i \<in> set (map fst bs). i < yid) \<and> (\<forall>i \<in> set (map fst cs). yid < i)"
-    using assms insert_ops_split \<open>insert_ops as1\<close> by blast
-  hence "ops = as @ [(xid, xr)] @ bs @ [(yid, yr)] @ cs"
-    using x_split by blast
-  moreover have "\<forall>i \<in> set (map fst bs). xid < i \<and> i < yid"
-    by (simp add: x_split y_split)
-  ultimately show ?thesis
-    using x_split y_split by blast
-qed
-
-lemma insert_ops_split_3:
-  assumes "insert_ops ops"
-    and "(xid, xr) \<in> set ops"
-    and "(yid, yr) \<in> set ops"
-    and "(zid, zr) \<in> set ops"
-    and "xid < yid" and "yid < zid"
-  shows "\<exists>as bs cs ds. ops = as @ [(xid, xr)] @ bs @ [(yid, yr)] @ cs @ [(zid, zr)] @ ds \<and>
-           (\<forall>i \<in> set (map fst as). i < xid) \<and>
-           (\<forall>i \<in> set (map fst bs). xid < i \<and> i < yid) \<and>
-           (\<forall>i \<in> set (map fst cs). yid < i \<and> i < zid) \<and>
-           (\<forall>i \<in> set (map fst ds). zid < i)"
-proof -
-  obtain as bs cs1 where xy_split: "ops = as @ [(xid, xr)] @ bs @ [(yid, yr)] @ cs1 \<and>
-           (\<forall>i \<in> set (map fst as). i < xid) \<and>
-           (\<forall>i \<in> set (map fst bs). xid < i \<and> i < yid) \<and>
-           (\<forall>i \<in> set (map fst cs1). yid < i)"
-    using assms insert_ops_split_2 by blast
-  hence "insert_ops ((as @ [(xid, xr)] @ bs @ [(yid, yr)]) @ cs1)"
-    using assms(1) by auto
-  hence "insert_ops cs1"
-    using assms(1) insert_ops_rem_prefix by blast
-  have "(zid, zr) \<in> set cs1"
-    using assms xy_split by auto
-  from this obtain cs ds where z_split: "cs1 = cs @ [(zid, zr)] @ ds \<and>
-      (\<forall>i \<in> set (map fst cs). i < zid) \<and> (\<forall>i \<in> set (map fst ds). zid < i)"
-    using assms insert_ops_split \<open>insert_ops cs1\<close> by blast
-  hence "ops = as @ [(xid, xr)] @ bs @ [(yid, yr)] @ cs @ [(zid, zr)] @ ds"
-    using xy_split by blast
-  moreover have "\<forall>i \<in> set (map fst cs). yid < i \<and> i < zid"
-    by (simp add: xy_split z_split)
-  ultimately show ?thesis
-    using xy_split z_split by blast
-qed
-
-lemma interp_list_last_None:
-  shows "oid \<in> set (interp_list (ops @ [(oid, None)]))"
-by (simp add: interp_list_tail_unfold)
-
-lemma interp_list_monotonic:
-  assumes "insert_ops (pre @ suf)"
-    and "oid \<in> set (interp_list pre)"
-  shows "oid \<in> set (interp_list (pre @ suf))"
-using assms interp_list_maybe_grow3 by auto
-
-lemma insert_ops_sorted_oids:
-  assumes "insert_ops (xs @ [(i1, r1)] @ ys @ [(i2, r2)])"
-  shows "i1 < i2"
-proof -
-  have "\<And>i. i \<in> set (map fst (xs @ [(i1, r1)] @ ys)) \<Longrightarrow> i < i2"
-    by (metis append.assoc assms last_op_greatest)
-  moreover have "i1 \<in> set (map fst (xs @ [(i1, r1)] @ ys))"
-    by auto
-  ultimately show "i1 < i2"
-    by blast
-qed
-
-lemma interp_list_append_non_memb:
-  assumes "insert_ops (pre @ [(oid, Some ref)] @ suf)"
-    and "ref \<notin> set (interp_list pre)"
-  shows "ref \<notin> set (interp_list (pre @ [(oid, Some ref)] @ suf))"
-using assms proof(induction suf rule: List.rev_induct)
-  case Nil
-  then show "ref \<notin> set (interp_list (pre @ [(oid, Some ref)] @ []))"
-    by (metis append_Nil2 insert_spec_nonex interp_list_tail_unfold)
-next
-  case (snoc x xs)
-  hence IH: "ref \<notin> set (interp_list (pre @ [(oid, Some ref)] @ xs))"
-    by (metis append_assoc insert_ops_rem_last)
-  moreover have "ref < oid"
-    using insert_ops_ref_older snoc.prems(1) by auto
-  moreover have "oid < fst x"
-    using insert_ops_sorted_oids by (metis prod.collapse snoc.prems(1))
-  have "set (interp_list ((pre @ [(oid, Some ref)] @ xs) @ [x])) =
-        set (interp_list (pre @ [(oid, Some ref)] @ xs)) \<or>
-        set (interp_list ((pre @ [(oid, Some ref)] @ xs) @ [x])) =
-        set (interp_list (pre @ [(oid, Some ref)] @ xs)) \<union> {fst x}"
-    by (metis (full_types) append.assoc interp_list_maybe_grow2 snoc.prems(1))
-  ultimately show "ref \<notin> set (interp_list (pre @ [(oid, Some ref)] @ xs @ [x]))"
-    using \<open>oid < fst x\<close> by auto
-qed
-
-lemma list_order_append:
-  assumes "insert_ops (pre @ suf)"
-    and "list_order pre x y"
-  shows "list_order (pre @ suf) x y"
-by (metis Un_iff assms list_order_monotonic insert_ops_appendD set_append subset_code(1))
-
-lemma list_order_insert_ref:
-  assumes "insert_ops (ops @ [(oid, Some ref)])"
-    and "ref \<in> set (interp_list ops)"
-  shows "list_order (ops @ [(oid, Some ref)]) ref oid"
-proof -
-  have "interp_list (ops @ [(oid, Some ref)]) = insert_spec (interp_list ops) (oid, Some ref)"
-    by (simp add: interp_list_tail_unfold)
-  moreover obtain xs ys where "interp_list ops = xs @ [ref] @ ys"
-    using assms(2) split_list_first by fastforce
-  hence "insert_spec (interp_list ops) (oid, Some ref) = xs @ [ref] @ [] @ [oid] @ ys"
-    using assms(1) insert_after_ref interp_list_distinct by fastforce
-  ultimately show "list_order (ops @ [(oid, Some ref)]) ref oid"
-    using assms(1) list_orderI by metis
-qed
-
-lemma list_order_insert_none:
-  assumes "insert_ops (ops @ [(oid, None)])"
-    and "x \<in> set (interp_list ops)"
-  shows "list_order (ops @ [(oid, None)]) oid x"
-proof -
-  have "interp_list (ops @ [(oid, None)]) = insert_spec (interp_list ops) (oid, None)"
-    by (simp add: interp_list_tail_unfold)
-  moreover obtain xs ys where "interp_list ops = xs @ [x] @ ys"
-    using assms(2) split_list_first by fastforce
-  hence "insert_spec (interp_list ops) (oid, None) = [] @ [oid] @ xs @ [x] @ ys"
-    by simp
-  ultimately show "list_order (ops @ [(oid, None)]) oid x"
-    using assms(1) list_orderI by metis
-qed
-
-lemma list_order_insert_between:
-  assumes "insert_ops (ops @ [(oid, Some ref)])"
-    and "list_order ops ref x"
-  shows "list_order (ops @ [(oid, Some ref)]) oid x"
-proof -
-  have "interp_list (ops @ [(oid, Some ref)]) = insert_spec (interp_list ops) (oid, Some ref)"
-    by (simp add: interp_list_tail_unfold)
-  moreover obtain xs ys zs where "interp_list ops = xs @ [ref] @ ys @ [x] @ zs"
-    using assms list_orderE by blast
-  moreover have "... = xs @ ref # (ys @ [x] @ zs)"
-    by simp
-  moreover have "distinct (xs @ ref # (ys @ [x] @ zs))"
-    using assms(1) calculation by (metis interp_list_distinct insert_ops_rem_last)
-  hence "insert_spec (xs @ ref # (ys @ [x] @ zs)) (oid, Some ref) = xs @ ref # oid # (ys @ [x] @ zs)"
-    using assms(1) calculation by (simp add: insert_after_ref)
-  moreover have "... = (xs @ [ref]) @ [oid] @ ys @ [x] @ zs"
-    by simp
-  ultimately show "list_order (ops @ [(oid, Some ref)]) oid x"
-    using assms(1) list_orderI by metis
-qed
-
-theorem no_interleaving:
-  assumes "insert_ops ops"
-    and "(xid, ref) \<in> set ops"
-    and "(yid, Some xid) \<in> set ops"
-    and "(zid, ref) \<in> set ops"
-    and "xid \<noteq> yid" and "yid \<noteq> zid" and "zid \<noteq> xid"
-  shows "(list_order ops xid yid \<and> list_order ops yid zid) \<or>
-         (list_order ops zid xid \<and> list_order ops xid yid) \<or>
-         (xid \<notin> set (interp_list ops) \<and> yid \<notin> set (interp_list ops) \<and>
-          zid \<notin> set (interp_list ops))"
-proof(cases "xid < zid")
-  case True
-  then show ?thesis
-  proof(cases "yid < zid")
-    case True
-    have "xid < yid"
-      using assms insert_ops_memb_ref_older by blast
-    then obtain as bs cs ds
-      where split: "ops = as @ [(xid, ref)] @ bs @ [(yid, Some xid)] @ cs @ [(zid, ref)] @ ds"
-      using assms \<open>yid < zid\<close> insert_ops_split_3 by blast
-    then show ?thesis
-    proof(cases ref)
-      case None
-      hence "xid \<in> set (interp_list (as @ [(xid, ref)]))"
-        using interp_list_last_None assms(1) split by metis
-      hence xid_in: "xid \<in> set (interp_list (as @ [(xid, ref)] @ bs))"
-        using interp_list_monotonic assms(1) insert_ops_appendD split append.assoc by metis
-      hence "list_order (as @ [(xid, ref)] @ bs @ [(yid, Some xid)]) xid yid"
-        using list_order_insert_ref assms(1) insert_ops_appendD split append.assoc by metis
-      hence "list_order ops xid yid"
-        using list_order_append assms(1) split append.assoc by metis
-      moreover have "xid \<in> set (interp_list (as @ [(xid, ref)] @ bs @ [(yid, Some xid)] @ cs))"
-        using interp_list_monotonic xid_in assms(1) insert_ops_appendD split append.assoc by metis
-      hence "list_order (as @ [(xid, ref)] @ bs @ [(yid, Some xid)] @ cs @ [(zid, ref)]) zid xid"
-        using list_order_insert_none assms(1) insert_ops_appendD split append.assoc None by metis
-      hence "list_order ops zid xid"
-        using list_order_append assms(1) split append.assoc by metis
-      ultimately show ?thesis by blast
-    next
-      case (Some r)
-      then show ?thesis
-      proof(cases "r \<in> set (interp_list as)")
-        case True
-        hence r_xid: "list_order (as @ [(xid, ref)]) r xid"
-          using list_order_insert_ref assms(1) insert_ops_appendD split append.assoc Some by metis
-        hence "xid \<in> set (interp_list (as @ [(xid, ref)]))"
-          using list_order_memb2 assms(1) split by metis
-        hence xid_in: "xid \<in> set (interp_list (as @ [(xid, ref)] @ bs))"
-          using interp_list_monotonic assms(1) insert_ops_appendD split append.assoc by metis
-        hence "list_order (as @ [(xid, ref)] @ bs @ [(yid, Some xid)]) xid yid"
-          using list_order_insert_ref assms(1) insert_ops_appendD split append.assoc by metis
-        hence "list_order ops xid yid"
-          using list_order_append assms(1) split append.assoc by metis
-        moreover have "list_order (as @ [(xid, ref)] @ bs @ [(yid, Some xid)] @ cs) r xid"
-          using list_order_append r_xid assms(1) insert_ops_appendD split append.assoc by metis
-        hence "list_order (as @ [(xid, ref)] @ bs @ [(yid, Some xid)] @ cs @ [(zid, ref)]) zid xid"
-          using list_order_insert_between assms(1) insert_ops_appendD split append.assoc Some by metis
-        hence "list_order ops zid xid"
-          using list_order_append assms(1) split append.assoc by metis
-        ultimately show ?thesis by blast
-      next
-        case False
-        hence "xid \<notin> set (interp_list ops)"
-          using interp_list_ref_nonex assms(1) split Some by metis
-        moreover have "xid \<notin> set (interp_list (as @ [(xid, ref)] @ bs))"
-          using interp_list_ref_nonex assms(1) insert_ops_appendD split append.assoc Some False by metis
-        hence "yid \<notin> set (interp_list ops)"
-          using interp_list_ref_nonex assms(1) split append.assoc by metis
-        moreover have "r \<notin> set (interp_list (as @ [(xid, ref)] @ bs @ [(yid, Some xid)] @ cs))"
-          using interp_list_append_non_memb assms(1) insert_ops_appendD split append.assoc Some False by metis
-        hence "zid \<notin> set (interp_list ops)"
-          using interp_list_ref_nonex assms(1) split append.assoc Some by metis
-        ultimately show ?thesis by blast
-      qed
-    qed
-  next
-    case False
-    hence "zid < yid"
-      using assms(6) by auto
-    then obtain as bs cs ds
-      where split: "ops = as @ [(xid, ref)] @ bs @ [(zid, ref)] @ cs @ [(yid, Some xid)] @ ds"
-      using assms \<open>xid < zid\<close> insert_ops_split_3 by blast
-    then show ?thesis
-    proof(cases ref)
-      case None
-      hence "xid \<in> set (interp_list (as @ [(xid, ref)]))"
-        using interp_list_last_None assms(1) split by metis
-      hence xid_in: "xid \<in> set (interp_list (as @ [(xid, ref)] @ bs))"
-        using interp_list_monotonic assms(1) insert_ops_appendD split append.assoc by metis
-      hence "list_order (as @ [(xid, ref)] @ bs @ [(zid, ref)]) zid xid"
-        using list_order_insert_none assms(1) insert_ops_appendD split append.assoc None by metis
-      hence "list_order ops zid xid"
-        using list_order_append assms(1) split append.assoc by metis
-      moreover have "xid \<in> set (interp_list (as @ [(xid, ref)] @ bs @ [(zid, ref)] @ cs))"
-        using interp_list_monotonic xid_in assms(1) insert_ops_appendD split append.assoc by metis
-      hence "list_order (as @ [(xid, ref)] @ bs @ [(zid, ref)] @ cs @ [(yid, Some xid)]) xid yid"
-        using list_order_insert_ref assms(1) insert_ops_appendD split append.assoc None by metis
-      hence "list_order ops xid yid"
-        using list_order_append assms(1) split append.assoc by metis
-      ultimately show ?thesis by blast
-    next
-      case (Some r)
-      then show ?thesis
-      proof(cases "r \<in> set (interp_list as)")
-        case True
-        hence r_xid: "list_order (as @ [(xid, ref)]) r xid"
-          using list_order_insert_ref assms(1) insert_ops_appendD split append.assoc Some by metis
-        hence "xid \<in> set (interp_list (as @ [(xid, ref)]))"
-          using list_order_memb2 assms(1) split by metis
-        hence xid_in: "xid \<in> set (interp_list (as @ [(xid, ref)] @ bs @ [(zid, ref)] @ cs))"
-          using interp_list_monotonic assms(1) insert_ops_appendD split append.assoc by metis
-        moreover have "list_order (as @ [(xid, ref)] @ bs) r xid"
-          using list_order_append r_xid assms(1) insert_ops_appendD split append.assoc by metis
-        hence "list_order (as @ [(xid, ref)] @ bs @ [(zid, ref)]) zid xid"
-          using list_order_insert_between assms(1) insert_ops_appendD split append.assoc Some by metis
-        hence "list_order ops zid xid"
-          using list_order_append assms(1) split append.assoc by metis
-        moreover have "list_order (as @ [(xid, ref)] @ bs @ [(zid, ref)] @ cs @ [(yid, Some xid)]) xid yid"
-          using list_order_insert_ref xid_in assms(1) insert_ops_appendD split append.assoc Some by metis
-        hence "list_order ops xid yid"
-          using list_order_append assms(1) split append.assoc by metis
-        ultimately show ?thesis by blast
-      next
-        case False
-        hence "xid \<notin> set (interp_list ops)"
-          using interp_list_ref_nonex assms(1) split Some by metis
-        moreover have "xid \<notin> set (interp_list (as @ [(xid, ref)] @ bs @ [(zid, ref)] @ cs))"
-          using interp_list_ref_nonex assms(1) insert_ops_appendD split append.assoc Some False by metis
-        hence "yid \<notin> set (interp_list ops)"
-          using interp_list_ref_nonex assms(1) split append.assoc by metis
-        moreover have "r \<notin> set (interp_list (as @ [(xid, ref)] @ bs))"
-          using interp_list_append_non_memb assms(1) insert_ops_appendD split append.assoc Some False by metis
-        hence "zid \<notin> set (interp_list ops)"
-          using interp_list_ref_nonex assms(1) split append.assoc Some by metis
-        ultimately show ?thesis by blast
-      qed
-    qed
-  qed
-next
-  case False
-  hence "zid < xid" and "xid < yid"
-    using assms neq_iff insert_ops_memb_ref_older by blast+
-  then obtain as bs cs ds
-    where split: "ops = as @ [(zid, ref)] @ bs @ [(xid, ref)] @ cs @ [(yid, Some xid)] @ ds"
-    using assms insert_ops_split_3 by blast
-  then show ?thesis
-  proof(cases ref)
-    case None
-    hence "zid \<in> set (interp_list (as @ [(zid, ref)]))"
-      using interp_list_last_None assms(1) split by metis
-    hence "zid \<in> set (interp_list (as @ [(zid, ref)] @ bs))"
-      using interp_list_monotonic assms(1) insert_ops_appendD split append.assoc by metis
-    hence xid_zid: "list_order (as @ [(zid, ref)] @ bs @ [(xid, ref)]) xid zid"
-      using list_order_insert_none assms(1) insert_ops_appendD split append.assoc None by metis
-    hence "list_order (as @ [(zid, ref)] @ bs @ [(xid, ref)] @ cs) xid zid"
-      using list_order_append assms(1) insert_ops_appendD split append.assoc by metis
-    hence "list_order (as @ [(zid, ref)] @ bs @ [(xid, ref)] @ cs @ [(yid, Some xid)]) yid zid"
-      using list_order_insert_between assms(1) insert_ops_appendD split append.assoc by metis
-    hence "list_order ops yid zid"
-      using list_order_append assms(1) split append.assoc by metis
-    moreover have "xid \<in> set (interp_list (as @ [(zid, ref)] @ bs @ [(xid, ref)]))"
-      using list_order_memb1 xid_zid assms(1) split by metis
-    hence "xid \<in> set (interp_list (as @ [(zid, ref)] @ bs @ [(xid, ref)] @ cs))"
-      using interp_list_monotonic assms(1) insert_ops_appendD split append.assoc by metis
-    hence "list_order (as @ [(zid, ref)] @ bs @ [(xid, ref)] @ cs @ [(yid, Some xid)]) xid yid"
-      using list_order_insert_ref assms(1) insert_ops_appendD split append.assoc by metis
-    hence "list_order ops xid yid"
-      using list_order_append assms(1) split append.assoc by metis
-    ultimately show ?thesis by blast
-  next
-    case (Some r)
-    then show ?thesis
-    proof(cases "r \<in> set (interp_list as)")
-      case True
-      hence "list_order (as @ [(zid, ref)]) r zid"
-        using list_order_insert_ref assms(1) insert_ops_appendD split append.assoc Some by metis
-      hence "list_order (as @ [(zid, ref)] @ bs) r zid"
-        using list_order_append assms(1) insert_ops_appendD split append.assoc by metis
-      hence "list_order (as @ [(zid, ref)] @ bs @ [(xid, ref)]) xid zid"
-        using list_order_insert_between assms(1) insert_ops_appendD split append.assoc Some by metis
-      hence xid_zid: "list_order (as @ [(zid, ref)] @ bs @ [(xid, ref)] @ cs) xid zid"
-        using list_order_append assms(1) insert_ops_appendD split append.assoc by metis
-      hence "list_order (as @ [(zid, ref)] @ bs @ [(xid, ref)] @ cs @ [(yid, Some xid)]) yid zid"
-        using list_order_insert_between assms(1) insert_ops_appendD split append.assoc by metis
-      hence "list_order ops yid zid"
-        using list_order_append assms(1) split append.assoc by metis
-      moreover have "xid \<in> set (interp_list (as @ [(zid, ref)] @ bs @ [(xid, ref)] @ cs))"
-        using list_order_memb1 xid_zid assms(1) split by metis
-      hence "list_order (as @ [(zid, ref)] @ bs @ [(xid, ref)] @ cs @ [(yid, Some xid)]) xid yid"
-        using list_order_insert_ref assms(1) insert_ops_appendD split append.assoc by metis
-      hence "list_order ops xid yid"
-        using list_order_append assms(1) split append.assoc by metis
-      ultimately show ?thesis by blast
-    next
-      case False
-      hence "zid \<notin> set (interp_list ops)"
-        using interp_list_ref_nonex assms(1) split Some by metis
-      moreover have r_notin: "r \<notin> set (interp_list (as @ [(zid, ref)] @ bs))"
-        using interp_list_append_non_memb assms(1) insert_ops_appendD split append.assoc Some False by metis
-      hence "xid \<notin> set (interp_list (as @ [(zid, ref)] @ bs @ [(xid, ref)] @ cs))"
-        using interp_list_ref_nonex assms(1) insert_ops_appendD split append.assoc Some by metis
-      hence "yid \<notin> set (interp_list ops)"
-        using interp_list_ref_nonex assms(1) split append.assoc by metis
-      moreover have "xid \<notin> set (interp_list ops)"
-        using interp_list_ref_nonex r_notin assms(1) split append.assoc Some by metis
-      ultimately show ?thesis by blast
-    qed
-  qed
-qed
 
 end
